Removed boolean variables because having to keep track of two substitutions was adding a lot of work

BasicConcrete.v
@@ -28,14 +28,12 @@ Inductive Aexpr : Type :=
 Inductive Bexpr : Type :=
 | BTrue
 | BFalse
-| BVar (x:string)
 | BNot (b:Bexpr)
 | BAnd (b1 b2:Bexpr)
 | BLeq (a1 a2:Aexpr).
 
 Coercion AVar : string >-> Aexpr.
 Coercion AConst : nat >-> Aexpr.
-Coercion BVar : string >-> Bexpr.
 
 Declare Custom Entry com.
 Declare Scope com_scope.
@@ -52,11 +50,89 @@ Definition X : string := "x".
 Definition Y : string := "y".
 Definition Z : string := "z".
 
+Open Scope com_scope.
+
+Definition sub : Type := string -> Aexpr.
+Definition id_sub : sub := fun x => x.
+Fixpoint Aapply (s:sub) (e:Aexpr) : Aexpr :=
+  match e with
+  | AConst n => AConst n
+  | AVar x => s x
+  | APlus a1 a2 => APlus (Aapply s a1) (Aapply s a2)
+  end.
+
+Lemma Aapply_id : forall e,
+    Aapply id_sub e = e.
+Proof.
+  induction e; try reflexivity.
+  simpl. rewrite IHe1. rewrite IHe2. reflexivity.
+Qed.
+
+Fixpoint Bapply  (s:sub) (e:Bexpr) : Bexpr :=
+  match e with
+  | BTrue => BTrue
+  | BFalse => BFalse
+  | BNot b => BNot (Bapply s b)
+  | BAnd b1 b2 => BAnd (Bapply s b1) (Bapply s b2)
+  | BLeq a1 a2 => BLeq (Aapply s a1) (Aapply s a2)
+  end.
+
+Definition update {E:Type} (s: string -> E) (x:string) (e:E) : string -> E :=
+  fun y => if String.eqb x y then e else s x.
+
+Lemma Bapply_id : forall e,
+    Bapply id_sub e = e.
+Proof.
+  induction e; simpl;
+    try (rewrite IHe);
+    try (rewrite IHe1; rewrite IHe2);
+    try (repeat rewrite Aapply_id);
+    try reflexivity.
+Qed.
+
+Definition Valuation := string -> nat.
+
+Fixpoint Aeval (V:Valuation) (e:Aexpr) : nat :=
+  match e with
+  | AConst n => n
+  | AVar x => V x
+  | APlus a1 a2 => (Aeval V a1) + (Aeval V a2)
+  end.
+
+Fixpoint Beval (V:Valuation) (e:Bexpr) : bool :=
+  match e with
+  | BTrue => true
+  | BFalse => false
+  | BNot b => negb (Beval V b)
+  | BAnd b1 b2 => (Beval V b1) && (Beval V b2)
+  | BLeq a1 a2 => (Aeval V a1) <=? (Aeval V a2)
+  end.
+
+Definition Comp (V:Valuation) (s:sub) : Valuation :=
+  fun x => Aeval V (s x).
+
+(** Lemma 2.1 *)
+Lemma comp_sub : forall V s e,
+    Aeval (Comp V s) e = Aeval V (Aapply s e).
+Proof.
+  induction e; simpl;
+  try (rewrite IHe1; rewrite IHe2); reflexivity.
+Qed.
+
+(* Corollary 2.2 *)
+Lemma asgn_sound : forall V s x e y,
+    Comp V (update s x (Aapply s e)) y = update (Comp V s) x (Aeval (Comp V s) e) y.
+Proof. intros. unfold Comp. unfold update. destruct (x =? y)%string;
+         try (rewrite <- comp_sub; unfold Comp);
+         reflexivity.
+Qed.
+
 Inductive Stmt : Type :=
 | SSkip
 | SAsgn (x:string) (e:Aexpr)
 | SSeq (s1 s2:Stmt)
-| SIf (b:Bexpr) (s1 s2:Stmt).
+| SIf (b:Bexpr) (s1 s2:Stmt)
+| SWhile (b:Bexpr) (s:Stmt).
 
 Notation "'skip'" := SSkip (in custom com at level 0) : com_scope.
 Notation "x := y"  :=
@@ -70,104 +146,14 @@ Notation "'if' x '{' y '}' '{' z '}'" :=
          (SIf x y z)
            (in custom com at level 89, x at level 99,
             y at level 99, z at level 99) : com_scope.
-Open Scope com_scope.
 
-Definition Asub : Type := string -> Aexpr.
-Definition Aid_sub : Asub := fun x => x.
-Fixpoint Aapply (s:Asub) (e:Aexpr) : Aexpr :=
-  match e with
-  | AConst n => AConst n
-  | AVar x => s x
-  | APlus a1 a2 => APlus (Aapply s a1) (Aapply s a2)
-  end.
+(** Symbolic semantics *)
 
-Lemma Aid_id : forall e,
-    Aapply Aid_sub e = e.
-Proof.
-  induction e; try reflexivity.
-  simpl. rewrite IHe1. rewrite IHe2. reflexivity.
-Qed.
+Definition SConfig : Type := Stmt * sub * Bexpr.
 
-Definition Bsub : Type := string -> Bexpr.
-Definition Bid_sub : Bsub := fun x => x.
-Fixpoint Bapply (s:Bsub) (s':Asub) (e:Bexpr) : Bexpr :=
-  match e with
-  | BTrue => BTrue
-  | BFalse => BFalse
-  | BVar x => s x
-  | BNot b => BNot (Bapply s s' b)
-  | BAnd b1 b2 => BAnd (Bapply s s' b1) (Bapply s s' b2)
-  | BLeq a1 a2 => BLeq (Aapply s' a1) (Aapply s' a2)
-  end.
+Reserved Notation " t '->s' t' " (at level 40).
 
-Definition update {E:Type} (s: string -> E) (x:string) (e:E) : string -> E :=
-  fun y => if String.eqb x y then e else s x.
-
-Lemma Bid_id : forall e,
-    Bapply Bid_sub Aid_sub e = e.
-Proof.
-  induction e; simpl;
-    try (rewrite IHe);
-    try (rewrite IHe1; rewrite IHe2);
-    try (repeat rewrite Aid_id);
-    reflexivity.
-Qed.
-
-Definition AValuation := string -> nat.
-Definition BValuation := string -> bool.
-
-Fixpoint Aeval (V:AValuation) (e:Aexpr) : nat :=
-  match e with
-  | AConst n => n
-  | AVar x => V x
-  | APlus a1 a2 => (Aeval V a1) + (Aeval V a2)
-  end.
-
-Fixpoint Beval (AV:AValuation) (BV:BValuation) (e:Bexpr) : bool :=
-  match e with
-  | BTrue => true
-  | BFalse => false
-  | BVar x => BV x
-  | BNot b => negb (Beval AV BV b)
-  | BAnd b1 b2 => (Beval AV BV b1) && (Beval AV BV b2)
-  | BLeq a1 a2 => (Aeval AV a1) <=? (Aeval AV a2)
-  end.
-
-Definition AComp (V:AValuation) (s:Asub) : AValuation :=
-  fun x => Aeval V (s x).
-
-Definition BComp (AV:AValuation) (BV:BValuation) (s:Bsub) : BValuation :=
-  fun x => Beval AV BV (s x).
-
-(** Lemma 2.1 (in two parts)*)
-Lemma comp_asub : forall V s e,
-    Aeval (AComp V s) e = Aeval V (Aapply s e).
-Proof.
-  induction e; simpl;
-  try (rewrite IHe1; rewrite IHe2); reflexivity.
-Qed.
-
-Lemma comp_bsub : forall AV BV s s' e,
-    Beval (AComp AV s') (BComp AV BV s) e = Beval AV BV (Bapply s s' e).
-Proof.
-  induction e; simpl;
-    try rewrite IHe;
-    try (rewrite IHe1; rewrite IHe2);
-    try (repeat rewrite comp_asub);
-    reflexivity.
-Qed.
-
-(* Corollary 2.2 *)
-Lemma asgn_soundA : forall V s x e y,
-    AComp V (update s x (Aapply s e)) y = update (AComp V s) x (Aeval (AComp V s) e) y.
-Proof. intros. unfold AComp. unfold update. destruct (x =? y)%string;
-         try (rewrite <- comp_asub; unfold AComp);
-         reflexivity.
-Qed.
-
-Lemma asgn_soundB : forall AV BV s s' x e y,
-    BComp AV BV (update s x (Bapply s s' e)) y = update (BComp AV BV s) x (Beval (AComp AV s') (BComp AV BV s) e) y.
-Proof. intros. unfold AComp. unfold BComp. unfold update. destruct (x =? y)%string;
-         try (rewrite <- comp_bsub; unfold BComp; unfold AComp);
-         reflexivity.
-Qed.
+Inductive Sstep : Relation SConfig :=
+| SAsgn_step : forall s x e sig phi,
+    (<{ x := e ; s }>, sig , phi) ->s (s, (update sig x e), phi)
+  where " t '->s' t' " := (Sstep t t').
